state monad redux

theories/exn.v
@@ -6,40 +6,40 @@ Section exceptions.
   Variables (E: Type).
 
   Inductive exn (A : Type) : Type :=
-  | Err (e: E)
+  | Exn (e: E)
   | OK (a: A).
-  Arguments Err {A} e.
+  Arguments Exn {A} e.
   Arguments OK {A} a.
 
   Definition exn_to_opt {A: Type} (c: exn A) : option A :=
     match c with
-    | Err _ => None
+    | Exn _ => None
     | OK a => Some a
     end.
 
   Definition exn_map {A B: Type} (f: A -> B) (c: exn A) : exn B :=
     match c with
-    | Err e => Err e
+    | Exn e => Exn e
     | OK a => OK (f a)
     end.
 
   Definition exn_bind {A B: Type} (f: A -> exn B) (c: exn A) : exn B :=
     match c with
-    | Err e => Err e
+    | Exn e => Exn e
     | OK a => f a
     end.
 
   Definition exn_join {A: Type} (c: exn (exn A)) : exn A :=
     match c with
     | OK (OK a) => OK a
-    | OK (Err e)
-    | Err e => Err e
+    | OK (Exn e)
+    | Exn e => Exn e
     end.
 
 End exceptions.
 
 Arguments OK {E A} _.
-Arguments Err {E A} _.
+Arguments Exn {E A} _.
 
 #[export]
 Instance exn_FMap {E} : FMap (exn E) := @exn_map E.
@@ -54,7 +54,7 @@ Instance exn_MRet {E} : MRet (exn E) := @OK E.
 Instance exn_MJoin {E} : MJoin (exn E) := @exn_join E.
 
 #[export]
-Instance exn_throw {E} : MThrow E (exn E) := @Err E.
+Instance exn_throw {E} : MThrow E (exn E) := @Exn E.
 
 Definition guard_opt {E A} (err: E) (c: option A) : exn E A :=
   match c with
